CellularAutomatas/open_questions.lean
@@ -12,8 +12,8 @@ namespace CellularAutomatas
 variable {α: Type} [Alphabet α]
 variable {Γ: Type} [Alphabet Γ]
 
--- open question: is every rt_closed advice a two-stage advice?
-theorem open_question_1 (adv: Advice α Γ) (h: adv.rt_closed): adv.is_two_stage_advice := by
+-- open question: is every weak_rt_closed advice a two-stage advice?
+theorem open_question_1 (adv: Advice α Γ) (h: adv.weak_rt_closed): adv.is_two_stage_advice := by
     sorry
 
 theorem lt_eq_rt: CA_rt α = CA_lt α := by
